coq/MapTerm.v
@@ -33,7 +33,7 @@ Definition map_operator {A B : Type} (f : A -> B) (a : list nat) (th : operator 
   | oper_cty _ => oper_cty _
   | oper_con _ => oper_con _
   | oper_karrow _ => oper_karrow _
-  | oper_arrow _ => oper_arrow _
+  | oper_tarrow _ => oper_tarrow _
   | oper_pi _ => oper_pi _
   | oper_clam _ => oper_clam _
   | oper_capp _ => oper_capp _
@@ -54,7 +54,7 @@ Definition map_operator {A B : Type} (f : A -> B) (a : list nat) (th : operator 
   | oper_eqtype _ => oper_eqtype _
   | oper_sequal _ => oper_sequal _
   | oper_subtype _ => oper_subtype _
-  | oper_kuniv _ => oper_kuniv _
+  | oper_kind _ => oper_kind _
   | oper_all _ => oper_all _
   | oper_alltp _ => oper_alltp _
   | oper_exist _ => oper_exist _
@@ -159,8 +159,8 @@ auto.
 Qed.
 
 
-Lemma map_arrow :
-  forall A B (f : A -> B) m1 m2, map_term f (arrow m1 m2) = arrow (map_term f m1) (map_term f m2).
+Lemma map_tarrow :
+  forall A B (f : A -> B) m1 m2, map_term f (tarrow m1 m2) = tarrow (map_term f m1) (map_term f m2).
 Proof.
 auto.
 Qed.
@@ -306,8 +306,8 @@ auto.
 Qed.
 
 
-Lemma map_kuniv :
-  forall A B (f : A -> B) m, map_term f (kuniv m) = kuniv (map_term f m).
+Lemma map_kind :
+  forall A B (f : A -> B) m, map_term f (kind m) = kind (map_term f m).
 Proof.
 auto.
 Qed.
@@ -495,7 +495,7 @@ auto.
 Qed.
 
 
-Hint Rewrite map_ext map_extt map_var map_univ map_cty map_con map_karrow map_arrow map_pi map_clam map_capp map_ctlam map_ctapp map_lam map_app map_intersect map_union map_fut map_cnext map_cprev map_next map_prev map_rec map_equal map_triv map_eqtype map_sequal map_subtype map_kuniv map_all map_alltp map_exist map_mu map_ispositive map_isnegative map_voidtp map_unittp map_cunit map_booltp map_btrue map_bfalse map_bite map_prod map_sigma map_cpair map_cpi1 map_cpi2 map_ppair map_ppi1 map_ppi2 map_wt map_set map_iset map_quotient map_guard : map.
+Hint Rewrite map_ext map_extt map_var map_univ map_cty map_con map_karrow map_tarrow map_pi map_clam map_capp map_ctlam map_ctapp map_lam map_app map_intersect map_union map_fut map_cnext map_cprev map_next map_prev map_rec map_equal map_triv map_eqtype map_sequal map_subtype map_kind map_all map_alltp map_exist map_mu map_ispositive map_isnegative map_voidtp map_unittp map_cunit map_booltp map_btrue map_bfalse map_bite map_prod map_sigma map_cpair map_cpi1 map_cpi2 map_ppair map_ppi1 map_ppi2 map_wt map_set map_iset map_quotient map_guard : map.
 
 
 Lemma map_sumbool :
